theories/typing/uninit.v
@@ -1,140 +1,14 @@
+Require Import FunctionalExtensionality.
 From iris.proofmode Require Import tactics.
 From lrust.typing Require Export type.
-From lrust.typing Require Import product.
 Set Default Proof Using "Type".
 
 Section uninit.
   Context `{!typeG Σ}.
 
-  Program Definition uninit_1 : type :=
-    {| st_lfts := []; st_E := []; st_own tid vl := ⌜length vl = 1%nat⌝%I |}.
-  Next Obligation. done. Qed.
+  Program Definition uninit (n: nat) : type unit :=
+    {| pt_size := n;  pt_own _ _ vl := ⌜length vl = n⌝%I |}.
+  Next Obligation. by iIntros. Qed.
+  Global Instance uninit_send n : Send (uninit n). Proof. done. Qed.
 
-  Global Instance uninit_1_send : Send uninit_1.
-  Proof. iIntros (depth tid1 tid2 vl) "H". done. Qed.
-
-  Definition uninit0 (n : nat) : type :=
-    Π (replicate n uninit_1).
-
-  Lemma uninit0_sz n : ty_size (uninit0 n) = n.
-  Proof. induction n=>//=. by f_equal. Qed.
-
-  Lemma uninit0_own n depth tid vl :
-    (uninit0 n).(ty_own) depth tid vl ⊣⊢ ⌜length vl = n⌝.
-  Proof.
-    iSplit.
-    - iIntros "Hvl".
-      iInduction n as [|n] "IH" forall (vl); simpl.
-      + by iDestruct "Hvl" as "->".
-      + iDestruct "Hvl" as (vl1 vl2) "(% & % & Hprod)".
-        destruct vl1 as [|v [|]]; try done. subst vl. simpl.
-        iDestruct ("IH" with "Hprod") as "%". iPureIntro. by f_equal.
-    - iIntros "<-". iInduction vl as [|v vl] "IH"=>//=. iExists [v], vl. auto.
-  Qed.
-
-  (* We redefine uninit as an alias of uninit0, so that ty_size and ty_own
-     compute directly.  We re-use the sharing from the product as that saves a whole
-     lot of work. *)
-  Program Definition uninit (n : nat) : type :=
-    {| ty_size := n; ty_lfts := []; ty_E := [];
-       ty_own depth tid vl := ⌜length vl = n⌝%I; ty_shr := (uninit0 n).(ty_shr) |}.
-  Next Obligation. iIntros (???) "%". done. Qed.
-  Next Obligation. iIntros (??????). auto. Qed.
-  Next Obligation.
-    iIntros (????????) "LFT _ Hvl".
-    iApply (ty_share (uninit0 n) with "LFT []"); first done.
-    { iInduction n as [|n] "IH"; [|done]. iApply lft_incl_static. }
-    iApply (bor_iff with "[] Hvl"). iIntros "!> !>". setoid_rewrite uninit0_own.
-    iSplit; iIntros; done.
-  Qed.
-  Next Obligation. intros. by apply ty_shr_mono. Qed.
-
-  Global Instance uninit_copy n : Copy (uninit n).
-  Proof.
-    assert (Copy (uninit0 n)) as [A B].
-    { apply product_copy. by apply Forall_replicate, _. }
-    split; first by apply _.
-    rewrite uninit0_sz in B. setoid_rewrite uninit0_own in B. done.
-  Qed.
-
-  Global Instance uninit_send n : Send (uninit n).
-  Proof. iIntros (????) "?". done. Qed.
-
-  Global Instance uninit_sync n : Sync (uninit n).
-  Proof. apply product_sync, Forall_replicate, _. Qed.
-
-  (* Unfolding lemma, kep only for backwards compatibility. *)
-  Lemma uninit_own n depth tid vl :
-    (uninit n).(ty_own) depth tid vl ⊣⊢ ⌜length vl = n⌝.
-  Proof. done. Qed.
-
-  Lemma uninit_uninit0_eqtype E L n :
-    eqtype E L (uninit0 n) (uninit n).
-  Proof.
-    apply eqtype_unfold. iIntros (qL) "_ !> _".
-    iSplit; [|iSplit; [|iSplit; iModIntro]].
-    - auto using uninit0_sz.
-    - induction n as [|n IH]=>//. iApply lft_equiv_refl.
-    - iIntros (???). by rewrite uninit0_own.
-    - iIntros (???). by iApply (bi.iff_refl True%I).
-  Qed.
-
-  Lemma uninit_product_subtype_cons_r {E L} (n : nat) ty tyl :
-    ty.(ty_size) ≤ n →
-    subtype E L (uninit ty.(ty_size)) ty →
-    subtype E L (uninit (n-ty.(ty_size))) (Π tyl) →
-    subtype E L (uninit n) (Π(ty :: tyl)).
-  Proof.
-    intros ?%Nat2Z.inj_le. rewrite -!uninit_uninit0_eqtype /uninit0=>Hty Htyl.
-    rewrite (le_plus_minus ty.(ty_size) n) // replicate_plus
-           -(prod_flatten_r _ _ [_]) /= -prod_app. repeat (done || f_equiv).
-  Qed.
-  Lemma uninit_product_subtype_cons_l {E L} (n : nat) ty tyl :
-    ty.(ty_size) ≤ n →
-    subtype E L ty (uninit ty.(ty_size)) →
-    subtype E L (Π tyl) (uninit (n-ty.(ty_size))) →
-    subtype E L (Π(ty :: tyl)) (uninit n).
-  Proof.
-    intros ?%Nat2Z.inj_le. rewrite -!uninit_uninit0_eqtype /uninit0=>Hty Htyl.
-    rewrite (le_plus_minus ty.(ty_size) n) // replicate_plus
-           -(prod_flatten_r _ _ [_]) /= -prod_app. repeat (done || f_equiv).
-  Qed.
-  Lemma uninit_product_eqtype_cons_r {E L} (n : nat) ty tyl :
-    ty.(ty_size) ≤ n →
-    eqtype E L (uninit ty.(ty_size)) ty →
-    eqtype E L (uninit (n-ty.(ty_size))) (Π tyl) →
-    eqtype E L (uninit n) (Π(ty :: tyl)).
-  Proof.
-    intros ? [] []. split.
-    - by apply uninit_product_subtype_cons_r.
-    - by apply uninit_product_subtype_cons_l.
-  Qed.
-  Lemma uninit_product_eqtype_cons_l {E L} (n : nat) ty tyl :
-    ty.(ty_size) ≤ n →
-    eqtype E L ty (uninit ty.(ty_size)) →
-    eqtype E L (Π tyl) (uninit (n-ty.(ty_size))) →
-    eqtype E L (Π(ty :: tyl)) (uninit n).
-  Proof. symmetry. by apply uninit_product_eqtype_cons_r. Qed.
-
-  Lemma uninit_unit_eqtype E L n :
-    n = 0%nat →
-    eqtype E L (uninit n) unit.
-  Proof. rewrite -uninit_uninit0_eqtype=>->//. Qed.
-  Lemma uninit_unit_eqtype' E L n :
-    n = 0%nat →
-    eqtype E L unit (uninit n).
-  Proof. rewrite -uninit_uninit0_eqtype=>->//. Qed.
-  Lemma uninit_unit_subtype E L n :
-    n = 0%nat →
-    subtype E L (uninit n) unit.
-  Proof. rewrite -uninit_uninit0_eqtype=>->//. Qed.
-  Lemma uninit_unit_subtype' E L n :
-    n = 0%nat →
-    subtype E L unit (uninit n).
-  Proof. rewrite -uninit_uninit0_eqtype=>->//. Qed.
 End uninit.
-
-Global Hint Resolve uninit_product_eqtype_cons_l uninit_product_eqtype_cons_r
-             uninit_product_subtype_cons_l uninit_product_subtype_cons_r
-             uninit_unit_eqtype uninit_unit_eqtype'
-             uninit_unit_subtype uninit_unit_subtype' : lrust_typing.
